Even more renaming along the same lines as last commit

ConvolutionalCodes/state_machineScript.sml
@@ -236,13 +236,15 @@ Definition transition_inverse_def:
   FILTER (λorgn. (m.transition_fn orgn).destination = dest) (all_transitions m)
 End
 
-Definition code_to_path_helper_def:
-  code_to_path_helper m [] s = [s] ∧
-  code_to_path_helper m (b::bs) s =  s::(code_to_path_helper m bs (vd_step m b s))
+
+
+Definition code_to_path_from_state_def:
+  code_to_path_from_state m [] s = [s] ∧
+  code_to_path_from_state m (b::bs) s =  s::(code_to_path_from_state m bs (vd_step m b s))
 End
 
 Definition code_to_path_def:
-  code_to_path m bs = code_to_path_helper m bs 0
+  code_to_path m bs = code_to_path_from_state m bs 0
 End
 
 (* -------------------------------------------------------------------------- *)
@@ -294,7 +296,7 @@ Definition path_is_valid_def:
 End
 
 Definition path_is_valid_from_state_def:
-  path_is_valid_from_state m ps s = ∃bs. code_to_path_helper m bs s = ps
+  path_is_valid_from_state m ps s = ∃bs. code_to_path_from_state m bs s = ps
 End
 
 Definition path_is_valid_or_empty_def:
@@ -771,44 +773,44 @@ Proof
   >> gvs[vd_step_tran_def]
 QED
         
-Theorem code_to_path_helper_hd:
+Theorem code_to_path_from_state_hd:
   ∀m bs s.
-  HD (code_to_path_helper m bs s) = s
+  HD (code_to_path_from_state m bs s) = s
 Proof
   Induct_on ‘bs’
   >- (rpt strip_tac >> EVAL_TAC)
   >> rpt strip_tac
-  >> gvs[code_to_path_helper_def]
+  >> gvs[code_to_path_from_state_def]
 QED
 
 Theorem code_to_path_hd:
   ∀m bs.
   HD (code_to_path m bs) = 0
 Proof
-  gvs[code_to_path_helper_hd, code_to_path_def]
+  gvs[code_to_path_from_state_hd, code_to_path_def]
 QED
 
-Theorem code_to_path_helper_null[simp]:
+Theorem code_to_path_from_state_null[simp]:
   ∀m bs s.
-  ¬NULL (code_to_path_helper m bs s)
+  ¬NULL (code_to_path_from_state m bs s)
 Proof
   rpt strip_tac
   >> Cases_on ‘bs’
-  >> gvs[code_to_path_helper_def]
+  >> gvs[code_to_path_from_state_def]
 QED
 
 Theorem code_to_path_null[simp]:
   ∀m bs.
   ¬NULL (code_to_path m bs)
 Proof
-  gvs[code_to_path_def, code_to_path_helper_null]
+  gvs[code_to_path_def, code_to_path_from_state_null]
 QED
 
-Theorem code_to_path_helper_length:
+Theorem code_to_path_from_state_length:
   ∀m bs s.
-  LENGTH (code_to_path_helper m bs s) = LENGTH bs + 1
+  LENGTH (code_to_path_from_state m bs s) = LENGTH bs + 1
 Proof
-  Induct_on ‘bs’ >> rpt strip_tac >> gvs[code_to_path_helper_def]
+  Induct_on ‘bs’ >> rpt strip_tac >> gvs[code_to_path_from_state_def]
 QED
 
 Theorem code_to_path_length:
@@ -816,32 +818,32 @@ Theorem code_to_path_length:
   LENGTH (code_to_path m bs) = LENGTH bs + 1
 Proof
   rpt strip_tac
-  >> gvs[code_to_path_def, code_to_path_helper_length] 
+  >> gvs[code_to_path_def, code_to_path_from_state_length] 
 QED
         
-Theorem code_to_path_helper_nonempty[simp]:
+Theorem code_to_path_from_state_nonempty[simp]:
   ∀m bs s.
-  code_to_path_helper m bs s ≠ []
+  code_to_path_from_state m bs s ≠ []
 Proof
   rpt strip_tac
-  >> gvs[GSYM NULL_EQ, code_to_path_helper_null]
+  >> gvs[GSYM NULL_EQ, code_to_path_from_state_null]
 QED
 
 Theorem code_to_path_nonempty[simp]:
   ∀m bs.
   code_to_path m bs ≠ []
 Proof
-  gvs[code_to_path_helper_nonempty, code_to_path_def]
+  gvs[code_to_path_from_state_nonempty, code_to_path_def]
 QED
 
-Theorem code_to_path_helper_append:
+Theorem code_to_path_from_state_append:
   ∀m bs cs s.
-  code_to_path_helper m (bs ⧺ cs) s = (code_to_path_helper m bs s) ⧺ (TL (code_to_path_helper m cs (vd_encode_state_from_state m bs s)))
+  code_to_path_from_state m (bs ⧺ cs) s = (code_to_path_from_state m bs s) ⧺ (TL (code_to_path_from_state m cs (vd_encode_state_from_state m bs s)))
 Proof
   Induct_on ‘bs’
   >- (EVAL_TAC
       >> rpt strip_tac
-      >> qspecl_then [‘m’, ‘cs’, ‘s’] assume_tac code_to_path_helper_hd
+      >> qspecl_then [‘m’, ‘cs’, ‘s’] assume_tac code_to_path_from_state_hd
       >> qmatch_goalsub_abbrev_tac ‘TL donotrewrite’
       >> last_x_assum (fn th => PURE_ONCE_REWRITE_TAC[GSYM th])
       >> unabbrev_all_tac
@@ -849,26 +851,26 @@ Proof
       >> gvs[])
   >> rpt strip_tac
   >> gvs[]
-  >> gvs[code_to_path_helper_def]
+  >> gvs[code_to_path_from_state_def]
   >> gvs[vd_encode_state_from_state_def]
 QED
 
-Theorem code_to_path_helper_snoc:
+Theorem code_to_path_from_state_snoc:
   ∀m b bs s.
-  code_to_path_helper m (SNOC b bs) s = SNOC (vd_step m b (vd_encode_state_from_state m bs s)) (code_to_path_helper m bs s)
+  code_to_path_from_state m (SNOC b bs) s = SNOC (vd_step m b (vd_encode_state_from_state m bs s)) (code_to_path_from_state m bs s)
 Proof
   rpt strip_tac
   >> gvs[SNOC]
-  >> gvs[code_to_path_helper_append]
-  >> gvs[code_to_path_helper_def]
+  >> gvs[code_to_path_from_state_append]
+  >> gvs[code_to_path_from_state_def]
 QED
 
 Theorem code_to_path_append:
   ∀m bs cs.
-  code_to_path m (bs ⧺ cs) = (code_to_path m bs) ⧺ (TL (code_to_path_helper m cs (vd_encode_state m bs)))
+  code_to_path m (bs ⧺ cs) = (code_to_path m bs) ⧺ (TL (code_to_path_from_state m cs (vd_encode_state m bs)))
 Proof
   rpt strip_tac
-  >> gvs[code_to_path_def, code_to_path_helper_append, vd_encode_state_def]
+  >> gvs[code_to_path_def, code_to_path_from_state_append, vd_encode_state_def]
 QED
 
 Theorem code_to_path_snoc:
@@ -877,19 +879,19 @@ Theorem code_to_path_snoc:
 Proof
   rpt strip_tac
   >> PURE_REWRITE_TAC[code_to_path_def]
-  >> PURE_REWRITE_TAC[code_to_path_helper_snoc]
+  >> PURE_REWRITE_TAC[code_to_path_from_state_snoc]
   >> gvs[]
   >> gvs[vd_encode_state_def]
 QED
 
-Theorem code_to_path_helper_last:
+Theorem code_to_path_from_state_last:
   ∀m bs s.
-  LAST (code_to_path_helper m bs s) = (vd_encode_state_from_state m bs s)
+  LAST (code_to_path_from_state m bs s) = (vd_encode_state_from_state m bs s)
 Proof
   Induct_on ‘bs’ >> rpt strip_tac
   >- EVAL_TAC
   >> gvs[vd_encode_state_from_state_def]
-  >> gvs[code_to_path_helper_def]
+  >> gvs[code_to_path_from_state_def]
   >> pop_assum $ qspecl_then [‘m’, ‘vd_step m h s’] assume_tac
   >> pop_assum (fn th => gvs[SYM th])
   >> gvs[LAST_DEF]
@@ -899,58 +901,58 @@ Theorem code_to_path_last:
   ∀m bs.
   LAST (code_to_path m bs) = (vd_encode_state m bs)
 Proof
-  gvs[code_to_path_helper_last, code_to_path_def, vd_encode_state_def]
+  gvs[code_to_path_from_state_last, code_to_path_def, vd_encode_state_def]
 QED
 
-Theorem code_to_path_helper_vd_can_step_cons:
+Theorem code_to_path_from_state_vd_can_step_cons:
   ∀m bs p p' ps s.
-  code_to_path_helper m bs s = p::p'::ps ⇒
+  code_to_path_from_state m bs s = p::p'::ps ⇒
   vd_can_step m p p'
 Proof
   rpt strip_tac
   >> Cases_on ‘bs’
-  >- gvs[code_to_path_def, code_to_path_helper_def]
-  >> gvs[code_to_path_def, code_to_path_helper_def]
+  >- gvs[code_to_path_def, code_to_path_from_state_def]
+  >> gvs[code_to_path_def, code_to_path_from_state_def]
   >> Cases_on ‘t’
-  >- (gvs[code_to_path_def, code_to_path_helper_def]
+  >- (gvs[code_to_path_def, code_to_path_from_state_def]
       >> gvs[vd_can_step_def]
       >> qexists ‘h’
       >> gvs[])
-  >> gvs[code_to_path_helper_def]
+  >> gvs[code_to_path_from_state_def]
   >> gvs[vd_can_step_def]
   >> qexists ‘h’
   >> gvs[]
 QED
 
-Theorem code_to_path_helper_vd_can_step:
+Theorem code_to_path_from_state_vd_can_step:
   ∀m bs p p' ps ps' s.
-  code_to_path_helper m bs s = (ps ⧺ [p; p'] ⧺ ps') ⇒
+  code_to_path_from_state m bs s = (ps ⧺ [p; p'] ⧺ ps') ⇒
   vd_can_step m p p'
 Proof
   Induct_on ‘ps’
   >- (rpt strip_tac
       >> gvs[]
-      >> irule code_to_path_helper_vd_can_step_cons
+      >> irule code_to_path_from_state_vd_can_step_cons
       >> qexistsl [‘bs’, ‘ps'’, ‘s’]
       >> gvs[]
      )
   >> rpt strip_tac
   >> last_x_assum irule
   >> Cases_on ‘bs’
-  >- gvs[code_to_path_def, code_to_path_helper_def]
+  >- gvs[code_to_path_def, code_to_path_from_state_def]
   >> gvs[]
-  >> gvs[code_to_path_def, code_to_path_helper_def]
+  >> gvs[code_to_path_def, code_to_path_from_state_def]
   >> qexistsl [‘t’, ‘ps'’, ‘vd_step m h' h’]
   >> gvs[]
 QED
 
-Theorem code_to_path_helper_vd_can_step_snoc:
+Theorem code_to_path_from_state_vd_can_step_snoc:
   ∀m bs p p' ps s.
-  code_to_path_helper m bs s  = SNOC p' (SNOC p ps) ⇒
+  code_to_path_from_state m bs s  = SNOC p' (SNOC p ps) ⇒
   vd_can_step m p p'
 Proof
   rpt strip_tac
-  >> irule code_to_path_helper_vd_can_step
+  >> irule code_to_path_from_state_vd_can_step
   >> qexistsl [‘bs’, ‘ps’, ‘[]’, ‘s’]
   >> gvs[]
 QED
@@ -960,7 +962,7 @@ Theorem code_to_path_vd_can_step_cons:
   code_to_path m bs = p::p'::ps ⇒
   vd_can_step m p p'
 Proof
-  metis_tac[code_to_path_def, code_to_path_helper_vd_can_step_cons]
+  metis_tac[code_to_path_def, code_to_path_from_state_vd_can_step_cons]
 QED
 
 Theorem code_to_path_vd_can_step:
@@ -968,7 +970,7 @@ Theorem code_to_path_vd_can_step:
   code_to_path m bs = (ps ⧺ [p; p'] ⧺ ps') ⇒
   vd_can_step m p p'
 Proof
-  metis_tac[code_to_path_def, code_to_path_helper_vd_can_step]
+  metis_tac[code_to_path_def, code_to_path_from_state_vd_can_step]
 QED
 
 Theorem code_to_path_vd_can_step_snoc:
@@ -976,7 +978,7 @@ Theorem code_to_path_vd_can_step_snoc:
   code_to_path m bs = SNOC p' (SNOC p ps) ⇒
   vd_can_step m p p'
 Proof
-  metis_tac[code_to_path_def, code_to_path_helper_vd_can_step_snoc]
+  metis_tac[code_to_path_def, code_to_path_from_state_vd_can_step_snoc]
 QED
 
 (* -------------------------------------------------------------------------- *)
@@ -1075,12 +1077,12 @@ Proof
   >> DEP_PURE_ONCE_REWRITE_TAC[path_to_code_append]
   >> gvs[]
   >> conj_tac
-  >- (gvs[code_to_path_helper_def])
+  >- (gvs[code_to_path_from_state_def])
   >> REVERSE conj_tac
-  >- (gvs[code_to_path_helper_def])
+  >- (gvs[code_to_path_from_state_def])
   >> gvs[code_to_path_def, vd_encode_state_def]
-  >> gvs[code_to_path_helper_def]
-  >> gvs[code_to_path_helper_last]
+  >> gvs[code_to_path_from_state_def]
+  >> gvs[code_to_path_from_state_last]
   >> DEP_PURE_ONCE_REWRITE_TAC[states_to_transition_input_vd_step]
   >> gvs[]
   >> irule vd_encode_state_from_state_is_valid
@@ -1289,28 +1291,28 @@ Proof
   >> gvs[path_is_connected_def, vd_can_step_def]
 QED
 
-Theorem path_is_connected_code_to_path_helper:
+Theorem path_is_connected_code_to_path_from_state:
   ∀m bs s.
-  path_is_connected m (code_to_path_helper m bs s)
+  path_is_connected m (code_to_path_from_state m bs s)
 Proof
   Induct_on ‘bs’
   >- (rpt strip_tac >> EVAL_TAC)
   >> rpt strip_tac
-  >> gvs[code_to_path_helper_def]
+  >> gvs[code_to_path_from_state_def]
   >> gvs[path_is_connected_cons1]
   >> pop_assum $ qspecl_then [‘m’, ‘vd_step m h s’] assume_tac
   >> qmatch_goalsub_abbrev_tac ‘(_::ps)’
   >> Cases_on ‘ps’
   >- gvs[]
   >> gvs[path_is_connected_cons]
-  >> Cases_on ‘bs’ >> gvs[code_to_path_helper_def]
+  >> Cases_on ‘bs’ >> gvs[code_to_path_from_state_def]
 QED
 
 Theorem path_is_connected_code_to_path:
   ∀m bs s.
   path_is_connected m (code_to_path m bs)
 Proof
-  gvs[path_is_connected_code_to_path_helper, code_to_path_def]
+  gvs[path_is_connected_code_to_path_from_state, code_to_path_def]
 QED
 
 Theorem path_is_valid_nonempty:
@@ -1336,30 +1338,30 @@ Proof
   >> EQ_TAC
   >- (rpt strip_tac 
       >- (gvs[path_is_valid_from_state_def]
-          >> gvs[path_is_connected_code_to_path_helper])
+          >> gvs[path_is_connected_code_to_path_from_state])
       >- gvs[path_is_valid_from_state_def]
       >> gvs[path_is_valid_from_state_def]
-      >> Cases_on ‘bs’ >> gvs[code_to_path_helper_def])
+      >> Cases_on ‘bs’ >> gvs[code_to_path_from_state_def])
   >> rpt strip_tac
   >> gvs[path_is_valid_from_state_def]
   >> Induct_on ‘ps’ using SNOC_INDUCT
   >- gvs[]
   >> rpt strip_tac
   >> Cases_on ‘ps’ using SNOC_CASES >> gvs[code_to_path_def, path_is_connected_def, path_is_valid_from_state_def]
-  >- (qexists ‘[]’ >> gvs[code_to_path_helper_def])
+  >- (qexists ‘[]’ >> gvs[code_to_path_from_state_def])
   >> gvs[path_is_connected_snoc]
   >> gs[vd_can_step_def]
   >> qexists ‘SNOC b bs’
   >> Cases_on ‘l’
   >- (gvs[path_is_connected_def]
       >> Cases_on ‘bs’
-      >> gvs[code_to_path_helper_def])
+      >> gvs[code_to_path_from_state_def])
   >> gvs[]
   >> PURE_REWRITE_TAC[GSYM SNOC_APPEND]
-  >> PURE_REWRITE_TAC[code_to_path_helper_snoc]
+  >> PURE_REWRITE_TAC[code_to_path_from_state_snoc]
   >> gvs[]
   >> AP_TERM_TAC
-  >> qspecl_then [‘m’, ‘bs’, ‘h’] assume_tac code_to_path_helper_last
+  >> qspecl_then [‘m’, ‘bs’, ‘h’] assume_tac code_to_path_from_state_last
   >> gvs[]
   >> pop_assum (fn th => PURE_REWRITE_TAC [GSYM th])
   >> gvs[LAST_DEF]
@@ -1434,12 +1436,12 @@ Proof
   >> gvs[path_is_valid_def]
   >> gvs[code_to_path_def]
   >> Cases_on ‘bs’
-  >- gvs[code_to_path_helper_def]
-  >> gvs[code_to_path_helper_def]
+  >- gvs[code_to_path_from_state_def]
+  >> gvs[code_to_path_from_state_def]
   >> Cases_on ‘t'’
-  >- (gvs[code_to_path_helper_def]
+  >- (gvs[code_to_path_from_state_def]
       >> qexists ‘h''’ >> gvs[])
-  >> gvs[code_to_path_helper_def]
+  >> gvs[code_to_path_from_state_def]
   >> qexists ‘h''’ >> gvs[]
 QED
 
@@ -1460,23 +1462,23 @@ Proof
   gvs[path_is_valid_or_empty_def, path_is_valid_code_to_path]
 QED
 
-Theorem code_to_path_helper_path_to_code:
+Theorem code_to_path_from_state_path_to_code:
   ∀m ps.
   ps ≠ [] ∧
   path_is_connected m ps ⇒
-  code_to_path_helper m (path_to_code m ps) (HD ps) = ps
+  code_to_path_from_state m (path_to_code m ps) (HD ps) = ps
 Proof
   rpt strip_tac
   >> Induct_on ‘ps’
   >- gvs[path_is_connected_def]
   >> rpt strip_tac
   >> Cases_on ‘ps’ >> gvs[]
-  >- gvs[code_to_path_def, code_to_path_helper_def]
+  >- gvs[code_to_path_def, code_to_path_from_state_def]
   >> drule path_is_connected_cons1
   >> rpt strip_tac
   >> gvs[]        
   >> gvs[path_to_code_def]
-  >> gvs[code_to_path_helper_def]
+  >> gvs[code_to_path_from_state_def]
   >> DEP_PURE_ONCE_REWRITE_TAC[vd_step_states_to_transition_input]
   >> gvs[]
   >> gvs[path_is_connected_def, vd_can_step_def]
@@ -1491,7 +1493,7 @@ Theorem code_to_path_path_to_code:
   path_is_connected m ps ⇒
   code_to_path m (path_to_code m ps) = ps
 Proof
-  metis_tac[code_to_path_def, code_to_path_helper_path_to_code]
+  metis_tac[code_to_path_def, code_to_path_from_state_path_to_code]
 QED
 
 Theorem vd_encode_state_from_state_path_to_code:
@@ -1502,9 +1504,9 @@ Theorem vd_encode_state_from_state_path_to_code:
   vd_encode_state_from_state m (path_to_code m ps) s = LAST ps
 Proof
   rpt strip_tac
-  >> qspecl_then [‘m’, ‘ps’] assume_tac code_to_path_helper_path_to_code
+  >> qspecl_then [‘m’, ‘ps’] assume_tac code_to_path_from_state_path_to_code
   >> Cases_on ‘ps’ >> gvs[]
-  >> gvs[GSYM code_to_path_helper_last]
+  >> gvs[GSYM code_to_path_from_state_last]
   >> gvs[path_is_valid_path_is_connected]
 QED
 
